sepcomp/linking_sim.v
@@ -62,17 +62,18 @@ Definition cast_ty (T1 T2: Type) (pf: T1=T2) (x : T1) : T2.
 rewrite pf in x; refine x.
 Defined. 
 
+Lemma types_eq {c : Core.t cores_S} {d : Core.t cores_T} (pf : c.(Core.i)=d.(Core.i)) : 
+  C (cores_T (Core.i d))=C (cores_T (Core.i c)).
+Proof. by rewrite pf. Qed.
+
+Notation cast pf x := (cast_ty (types_eq pf) x).
+
 Section frame_inv.
 
 Import Core.
 
 Variables (c : t cores_S) (d : t cores_T). 
 Variable  (pf : c.(i)=d.(i)).
-
-Lemma types_eq : C (cores_T (i d))=C (cores_T (i c)).
-Proof. by rewrite pf. Qed.
-
-Notation cast x := (cast_ty types_eq x).
 
 Require Import compcert.lib.Coqlib. (*for Forall2*)
 
@@ -82,11 +83,12 @@ Record frame_inv cd0 mu0 mu m10 m1 e1 ef_sig1 vals1 m20 m2 e2 ef_sig2 vals2 : Ty
   ; pubTgt' := fun b => [&& locBlocksTgt mu0 b & REACH m20 (exportedTgt mu0 vals2) b] 
   ; nu0     := replace_locals mu0 pubSrc' pubTgt'
 
-    (* invariants *)
+    (* invariants required to instantiate at_external *)
   ; frame_inj   : Mem.inject (as_inj mu0) m10 m20
-  ; frame_match : (sims c.(i)).(match_state) cd0 mu0 c.(Core.c) m10 (cast d.(Core.c)) m20 
-  ; frame_at1   : at_external (cores_S c.(i)).(coreSem) c.(Core.c)        = Some (e1, ef_sig1, vals1) 
-  ; frame_at2   : at_external (cores_T c.(i)).(coreSem) (cast d.(Core.c)) = Some (e2, ef_sig2, vals2) 
+  ; frame_match : (sims c.(i)).(match_state) cd0 mu0 c.(Core.c) m10 (cast pf d.(Core.c)) m20 
+  ; frame_at1   : at_external (cores_S c.(i)).(coreSem) c.(Core.c) = Some (e1, ef_sig1, vals1) 
+  ; frame_at2   : at_external (cores_T c.(i)).(coreSem) (cast pf d.(Core.c)) 
+                    = Some (e2, ef_sig2, vals2) 
   ; frame_vinj  : Forall2 (val_inject (as_inj mu0)) vals1 vals2  
 
   ; frame_fwd1  : mem_forward m10 m1
@@ -99,20 +101,60 @@ Record frame_inv cd0 mu0 mu m10 m1 e1 ef_sig1 vals1 m20 m2 e2 ef_sig2 vals2 : Ty
   ; frame_sep  : StructuredInjections.sm_inject_separated mu0 mu m10 m20 }.
 
 End frame_inv.
+
+Section head_inv.
+
+Import Core.
+
+Variables (c : t cores_S) (d : t cores_T). 
+Variable  (pf : c.(i)=d.(i)).
+
+Record head_inv cd mu m1 m2 : Type :=
+  { head_match : (sims c.(i)).(match_state) cd mu c.(Core.c) m1 (cast pf d.(Core.c)) m2 }.
+
+End head_inv.
     
-Fixpoint stack_inv mu (s1 : Stack.t (Core.t cores_S)) (s2 : Stack.t (Core.t cores_T)) m1 m2 :=
+Fixpoint tail_inv mu (s1 : Stack.t (Core.t cores_S)) (s2 : Stack.t (Core.t cores_T)) m1 m2 :=
   match s1, s2 with
     | c :: s1', d :: s2' => 
       [/\ exists (pf : c.(Core.i)=d.(Core.i)) cd0 mu0,
           exists m10 e1 ef_sig1 vals1,
           exists m20 e2 ef_sig2 vals2, 
             frame_inv c d pf cd0 mu0 mu m10 m1 e1 ef_sig1 vals1 m20 m2 e2 ef_sig2 vals2
-        & stack_inv mu s1' s2' m1 m2]
+        & tail_inv mu s1' s2' m1 m2]
     | _, _ => False
   end.
 
-Let R (data : Lex.t types) mu (x1 : linker N cores_S) m1 (x2 : linker N cores_T) m2 := 
-  stack_inv mu x1.(Linker.stack).(CallStack.callStack) x2.(Linker.stack).(CallStack.callStack) m1 m2. 
+Section R.
+
+Import CallStack.
+Import Linker.
+
+Record R (data : Lex.t types) mu (x1 : linker N cores_S) m1 (x2 : linker N cores_T) m2 := 
+  { (* local defns. *)
+    s1  := x1.(stack) 
+  ; s2  := x2.(stack) 
+  ; pf1 := CallStack.callStack_nonempty s1 
+  ; pf2 := CallStack.callStack_nonempty s2 
+  ; c   := stack.head _ pf1 
+  ; d   := stack.head _ pf2 
+    (* invariants *)
+  ; R_head : exists (pf : c.(Core.i)=d.(Core.i)) cd, head_inv c d pf cd mu m1 m2 
+  ; R_tail : tail_inv mu s1.(callStack) s2.(callStack) m1 m2 }.
+
+End R.
+
+Section R_defs.
+
+Context data mu x1 m1 x2 m2 (pf : R data mu x1 m1 x2 m2).
+
+Lemma R_wd : SM_wd mu.
+Proof. 
+move: (R_head pf)=> [A][B]; move/head_match.
+by apply: (match_sm_wd _ _ _ _ _ (sims (Core.i (c pf)))).
+Qed.
+
+End R_defs.
 
 Lemma link : SM_simulation_inject linker_S linker_T my_ge my_ge entry_points.
 Proof.
@@ -125,6 +167,11 @@ eapply Build_SM_simulation_inject
 (* well_founded ord *)
 - by apply: Lex.wf_ord.
 
+(* match -> SM_wd mu *)
+- by apply: R_wd. 
+
 Admitted. (*WORK-IN-PROGRESS*)
 
 End linkingSimulation.
+
+
